ET instances extra args removed

txn-data-consistency/Execution_Tests.thy
@@ -24,48 +24,48 @@ definition R_onK :: "'v dep_rel \<Rightarrow> 'v kv_store \<Rightarrow> txid rel
 
 subsection \<open>Consistency models' execution tests\<close>
 
-definition R_CC :: "'v kv_store \<Rightarrow> 'v fingerpr \<Rightarrow> txid rel" where
-  "R_CC K F \<equiv> SO \<union> R_onK WR K"
+definition R_CC :: "'v kv_store \<Rightarrow> txid rel" where
+  "R_CC K \<equiv> SO \<union> R_onK WR K"
 
 definition R_UA :: "'v kv_store \<Rightarrow> 'v fingerpr \<Rightarrow> txid rel" where
   "R_UA K F \<equiv> \<Union>k. if W \<in> dom (F k) then (WW K k)^-1 else {}"
 
 definition R_PSI :: "'v kv_store \<Rightarrow> 'v fingerpr \<Rightarrow> txid rel" where
-  "R_PSI K F \<equiv> R_UA K F \<union> R_CC K F \<union> R_onK WW K"
+  "R_PSI K F \<equiv> R_UA K F \<union> R_CC K \<union> R_onK WW K"
 
-definition R_CP :: "'v kv_store \<Rightarrow> 'v fingerpr \<Rightarrow> txid rel" where
-  "R_CP K F \<equiv> SO O (R_onK RW K)^= \<union> (R_onK WR K) O (R_onK RW K)^= \<union> (R_onK WW K)"
+definition R_CP :: "'v kv_store \<Rightarrow> txid rel" where
+  "R_CP K \<equiv> SO O (R_onK RW K)^= \<union> (R_onK WR K) O (R_onK RW K)^= \<union> (R_onK WW K)"
 
 definition R_SI :: "'v kv_store \<Rightarrow> 'v fingerpr \<Rightarrow> txid rel" where
-  "R_SI K F \<equiv> R_UA K F \<union> R_CP K F \<union> (R_onK WW K) O (R_onK RW K)"
+  "R_SI K F \<equiv> R_UA K F \<union> R_CP K \<union> (R_onK WW K) O (R_onK RW K)"
 
-definition R_SER :: "'v kv_store \<Rightarrow> 'v fingerpr \<Rightarrow> txid rel" where
-  "R_SER K F \<equiv> (R_onK WW K)^-1"
+definition R_SER :: "'v kv_store \<Rightarrow> txid rel" where
+  "R_SER K \<equiv> (R_onK WW K)^-1"
 
-definition vShift_MR :: "'v kv_store \<Rightarrow> view \<Rightarrow> 'v kv_store \<Rightarrow> view \<Rightarrow> bool" where
-  "vShift_MR K u K' u' \<equiv> u \<sqsubseteq> u'"
+definition vShift_MR :: "view \<Rightarrow> view \<Rightarrow> bool" where
+  "vShift_MR u u' \<equiv> u \<sqsubseteq> u'"
 
 definition vShift_RYW :: "'v kv_store \<Rightarrow> view \<Rightarrow> 'v kv_store \<Rightarrow> view \<Rightarrow> bool" where
   "vShift_RYW K u K' u' \<equiv>
     \<forall>t \<in> kvs_txids K' - kvs_txids K. \<forall>k i. (v_writer (K' k!i) , t) \<in> SO^= \<longrightarrow> i \<in> u' k"
 
 definition vShift_MR_RYW :: "'v kv_store \<Rightarrow> view \<Rightarrow> 'v kv_store \<Rightarrow> view \<Rightarrow> bool" where
-  "vShift_MR_RYW K u K' u' \<equiv> vShift_MR K u K' u' \<and> vShift_RYW K u K' u'"
+  "vShift_MR_RYW K u K' u' \<equiv> vShift_MR u u' \<and> vShift_RYW K u K' u'"
 
-interpretation ET_MR: ExecutionTest "\<lambda>K F. {}" vShift_MR .
+interpretation ET_MR: ExecutionTest "\<lambda>K F. {}" "\<lambda>K u K' u'. vShift_MR u u'" .
 
 interpretation ET_RYW: ExecutionTest "\<lambda>K F. {}"  vShift_RYW .
 
-interpretation ET_CC: ExecutionTest R_CC vShift_MR_RYW .
+interpretation ET_CC: ExecutionTest "\<lambda>K F. R_CC K" vShift_MR_RYW .
 
 interpretation ET_UA: ExecutionTest R_UA "\<lambda>K u K' u'. True" .
 
 interpretation ET_PSI: ExecutionTest R_PSI vShift_MR_RYW .
 
-interpretation ET_CP: ExecutionTest R_CP vShift_MR_RYW .
+interpretation ET_CP: ExecutionTest "\<lambda>K F. R_CP K" vShift_MR_RYW .
 
 interpretation ET_SI: ExecutionTest R_SI vShift_MR_RYW .
 
-interpretation ET_SER: ExecutionTest R_SER "\<lambda>K u K' u'. True" .
+interpretation ET_SER: ExecutionTest "\<lambda>K F. R_SER K" "\<lambda>K u K' u'. True" .
 
 end
